proof/DDC/Language/SystemF2/TySubsts.v
@@ -1,0 +1,224 @@
+
+
+Require Export DDC.Language.SystemF2.TyBase.
+Require Export DDC.Language.SystemF2.TyLift.
+Require Import Coq.Logic.FunctionalExtensionality.
+
+
+Definition substTTs' (ix: nat) (d: nat) (us: list ty) (tt: ty)
+ := match get (ix - d) us with
+    | Some u => u
+    | None   => TVar (ix - length us)
+   end.
+
+Fixpoint substTTs (d: nat) (us: list ty) (tt: ty)
+ := match tt with
+   |  TVar ix
+   => match nat_compare ix d with
+      | Lt => TVar ix   (* ix is locally bound *)
+      | _  => substTTs' ix d us tt
+      end
+
+   |  TCon _
+   => tt
+   
+   |  TForall t
+   => TForall (substTTs (S d) (map (liftTT 1 0) us) t)
+
+   |  TApp t1 t2
+   => TApp (substTTs d us t1) (substTTs d us t2)
+   end.
+
+
+(********************************************************************)
+Lemma substTTs_makeTApps 
+ :  forall d us t1 ts
+ ,  substTTs d us (makeTApps t1 ts) 
+ =  makeTApps (substTTs d us t1) (map (substTTs d us) ts).
+Proof.
+ intros. gen d us t1.
+ induction ts; intros.
+  auto.
+  simpl. rewrite IHts. auto.
+Qed.
+
+
+Ltac fbreak_get 
+ := match goal with 
+    |  [ |- context [get ?E1 ?E2] ] 
+    => case (get E1 E2)
+    end.
+
+Ltac fbreak_le_gt_dec
+ := match goal with 
+     |  [ |- context [le_gt_dec ?n ?n'] ]
+     => case (le_gt_dec n n')
+    end.
+
+
+Ltac lift_unfold := 
+ repeat (intros; simpl;
+  first [ fbreak_nat_compare
+        | fbreak_le_gt_dec
+        | fbreak_get]).
+
+
+Lemma match_option
+ : forall {A} {B} (f: A -> B) (xs: list A) ix y
+ , f (match get ix xs         with | Some x => x | None  => y   end)
+ =   (match get ix (map f xs) with | Some x => x | None  => f y end).
+Proof.
+ intros.
+ remember (get ix xs) as Get.
+ destruct Get.
+  symmetry in HeqGet.
+  apply (get_map f) in HeqGet.
+  rewrite HeqGet. auto.
+
+  admit. (* fine, list lemma *)
+Qed.
+
+
+Lemma get_none_length
+ :  forall {A} n (xs: list A)
+ ,  get n xs = None
+ -> length xs <= n.
+Proof.
+ intros. gen n.
+ induction xs; intros.
+  simpl. burn.
+  simpl. simpl in H.
+   destruct n.
+    false.
+    apply IHxs in H. omega.
+Qed.
+
+
+
+(********************************************************************)
+(* Lifting after substitution *)
+Lemma liftTT_substTTs_1
+ :  forall n n' t1 us
+ ,  liftTT 1 n (substTTs (n + n') us t1)
+ =  substTTs (1 + n + n') (map (liftTT 1 n) us) (liftTT 1 n t1).
+Proof.
+ intros. gen n n' us.
+ induction t1; intros.
+
+ Case "TCon".
+  auto.
+
+ Case "TVar".
+  lift_unfold; 
+   induction us; 
+    unfold substTTs';
+    try lift_unfold; intros; simpl;
+    try (rewrite map_length);
+    try burn.
+
+  SCase "manual case".
+   rrwrite (n0 + n' - (n0 + n') = 0).
+   rrwrite (n0 + n' + 1 - S (n0 + n') = 0). 
+   auto.
+
+  SCase "manual case".
+   nnat.
+   rrwrite  (S n - S (n0 + n') = n - (n0 + n')).
+   remember (n - (n0 + n')) as X.
+   destruct X.
+    auto.
+    rewrite (match_option (liftTT 1 n0)).
+    simpl.
+    remember (get X (map (liftTT 1 n0) us)) as Y.
+    destruct Y. 
+     auto. 
+     symmetry in HeqY.
+     apply get_none_length in HeqY.
+     rewrite map_length in HeqY.
+     lift_unfold; 
+      intros; fequal; burn.
+
+ Case "TForall".
+  simpl. f_equal. 
+  induction us.
+   simpl. 
+    rrwrite (S (n + n') = (S n) + n').
+    rewrite IHt1. auto.
+
+   simpl.
+    rewrite (liftTT_liftTT_11 0 n). simpl.
+    rewrite (IHt1 (S n) n'). 
+    f_equal. simpl. f_equal.
+    rewrite map_map. rewrite map_map.
+    f_equal. unfold compose. 
+    extensionality x.
+    symmetry.
+    rrwrite (n = n + 0).
+    rewrite liftTT_liftTT. auto.
+
+ Case "TApp".
+  simpl. f_equal.
+  rewritess. rewritess.
+Qed.
+
+
+Lemma liftTT_substTTs
+ :  forall m n n' t1 us
+ ,  liftTT m n (substTTs (n + n') us t1)
+ =  substTTs (m + n + n') (map (liftTT m n) us) (liftTT m n t1).
+Proof.
+ intros. gen n n'.
+ induction m; intros.
+  simpl.
+   rewrite liftTT_zero.
+   rewrite liftTT_zero.
+   f_equal.
+   rewrite (@map_impl ty ty (liftTT 0 n) id).
+    induction us; auto. simpl. rewrite <- IHus. auto.
+   intros. rewrite liftTT_zero. unfold id. auto.
+
+  simpl.
+  rrwrite (S m = 1 + m).
+  rewrite <- liftTT_plus.
+  rewrite IHm.
+  simpl.
+  rrwrite (m + n + n' = n + (m + n')).
+  rewrite liftTT_substTTs_1.
+  f_equal.
+  rewrite map_map. unfold compose.
+  f_equal.
+  extensionality x.
+  rewrite -> liftTT_plus. auto.
+  rewrite -> liftTT_plus. auto.
+Qed.
+
+
+(********************************************************************)
+(* Lifting after substitution, 
+   with the lifting at a higher index *)
+(*
+Lemma liftTT_substTTs'
+ :  forall n n' t1 us
+ ,  length us > 0
+ -> liftTT 1 (n + n') (substTTs n us t1)
+ =  substTTs n (map (liftTT 1 (n + n')) us) (liftTT 1 (length us + n + n') t1).
+Proof.
+ intros. gen n n' us.
+ induction t1; intros.
+
+ Case "TCon".
+  simpl. auto.
+
+ Case "TVar".
+
+  repeat ( unfold liftTT; unfold substTTs; unfold substTTs';
+           fold   liftTT; fold substTTs; fold substTTs'
+         ; try fbreak_le_gt_dec
+         ; try fbreak_nat_compare
+         ; try fbreak_get
+         ; intros)
+    ; try (rewrite map_length)
+    ; try burn.
+
+ admit. admit. admit.
+*)
